theories/Monoids.v
@@ -1,7 +1,7 @@
 Require Import Coq.Relations.Relations.
-Require Import Coq.Classes.RelationClasses.
-Require Import Coq.Classes.Morphisms.
+From Coq.Classes Require Import RelationClasses Morphisms.
 From algebra Require Import Semigroups.
+Require Import Setoid.
 
 Section Monoids.
 Context {Carrier: Type}.
@@ -11,62 +11,54 @@ Context (op: Carrier -> Carrier -> Carrier).
 Context {op_proper: Proper (equiv ==> equiv ==> equiv) op}.
 Context (ident: Carrier).
 
-Infix "~" := equiv (at level 60, no associativity).
+Infix "==" := equiv (at level 60, no associativity).
 Infix "<o>" := op (at level 40, no associativity).
 
 Class Monoid := {
   monoid_semigroup :> Semigroup equiv op;
   monoid_ident_l:
-    forall (a: Carrier), ident <o> a ~ a;
+    forall (a: Carrier), ident <o> a == a;
   monoid_ident_r:
-    forall (a: Carrier), a <o> ident ~ a;
+    forall (a: Carrier), a <o> ident == a;
 }.
 
 Context {monoid: Monoid}.
 
 Theorem group_ident_l_unique (e: Carrier):
-  (forall (a: Carrier), e <o> a ~ a) ->
-  e ~ ident.
+  (forall (a: Carrier), e <o> a == a) ->
+  e == ident.
 Proof.
   intros Hl.
   specialize (Hl ident).
-  transitivity (e <o> ident);
-    [| assumption].
+  setoid_rewrite <- Hl.
   symmetry.
   apply monoid_ident_r.
 Qed.
 
 Theorem group_ident_r_unique (e: Carrier):
-  (forall (a: Carrier), a <o> e ~ a) ->
-  e ~ ident.
+  (forall (a: Carrier), a <o> e == a) ->
+  e == ident.
 Proof.
   intros Hr.
   specialize (Hr ident).
-  transitivity (ident <o> e);
-    [| assumption].
+  setoid_rewrite <- Hr.
   symmetry.
   apply monoid_ident_l.
 Qed.
 
-Definition monoid_op_l := semigroup_op_l equiv op.
 Lemma monoid_op_l_solo (a b: Carrier):
-  a ~ ident -> b <o> a ~ b.
+  a == ident -> b <o> a == b.
 Proof.
   intros H.
-  transitivity (b <o> ident);
-    [| apply monoid_ident_r].
-  apply monoid_op_l.
-  assumption.
+  setoid_rewrite H.
+  apply monoid_ident_r.
 Qed.
 
-Definition monoid_op_r := semigroup_op_r equiv op.
 Lemma monoid_op_r_solo (a b: Carrier):
-  a ~ ident -> a <o> b ~ b.
+  a == ident -> a <o> b == b.
 Proof.
   intros H.
-  transitivity (ident <o> b);
-    [| apply monoid_ident_l].
-  apply monoid_op_r.
-  assumption.
+  setoid_rewrite H.
+  apply monoid_ident_l.
 Qed.
 End Monoids.
