theories/Semigroups.v
@@ -1,6 +1,6 @@
 Require Import Coq.Relations.Relations.
-Require Import Coq.Classes.RelationClasses.
-Require Import Coq.Classes.Morphisms.
+From Coq.Classes Require Import RelationClasses Morphisms.
+Require Import Setoid.
 
 Section Semigroups.
 Context {Carrier: Type}.
@@ -9,37 +9,36 @@ Context {equiv_equiv: Equivalence equiv}.
 Context (op: Carrier -> Carrier -> Carrier).
 Context {op_proper: Proper (equiv ==> equiv ==> equiv) op}.
 
-Infix "~" := equiv (at level 60, no associativity).
+Infix "==" := equiv (at level 60, no associativity).
 Infix "<o>" := op (at level 40, left associativity).
 
 Class Semigroup := {
   semigroup_assoc:
     forall (a b c: Carrier),
-      a <o> b <o> c ~ a <o> (b <o> c);
+      a <o> b <o> c == a <o> (b <o> c);
 }.
 
 Context {semigroup: Semigroup}.
 
 Lemma semigroup_op_l (a b: Carrier):
-  a ~ b -> forall (c: Carrier), c <o> a ~ c <o> b.
+  a == b -> forall (c: Carrier), c <o> a == c <o> b.
 Proof.
   intros Hab c.
-  apply op_proper;
-    [reflexivity | assumption].
+  setoid_rewrite Hab.
+  reflexivity.
 Qed.
 
 Lemma semigroup_op_r (a b: Carrier):
-  a ~ b -> forall (c: Carrier), a <o> c ~ b <o> c.
+  a == b -> forall (c: Carrier), a <o> c == b <o> c.
 Proof.
   intros Hab c.
-  apply op_proper;
-    [assumption | reflexivity].
+  setoid_rewrite Hab.
+  reflexivity.
 Qed.
 
 Class Commutative := {
     commutative:
       forall (a b: Carrier),
-        a <o> b ~ b <o> a;
+        a <o> b == b <o> a;
 }.
 End Semigroups.
-
