theories/GroupIter.v
@@ -1,0 +1,459 @@
+Require Import Coq.Relations.Relations.
+From Coq.Classes Require Import RelationClasses Morphisms.
+Require Import Coq.PArith.PArith.
+Require Import Coq.ZArith.ZArith.
+From algebra Require Import Semigroups Monoids Groups.
+
+Section OpIterations.
+Context {Carrier: Type}.
+Context (equiv: relation Carrier).
+Context {equiv_equiv: Equivalence equiv}.
+Context (op: Carrier -> Carrier -> Carrier).
+Context {op_proper: Proper (equiv ==> equiv ==> equiv) op}.
+
+Definition semigroup_iter_op (p: positive)(a: Carrier): Carrier :=
+  Pos.iter_op op p a.
+
+Theorem semigroup_iter_op_proper:
+  Proper (eq ==> equiv ==> equiv) semigroup_iter_op.
+Proof.
+  intros m n ->.
+  induction n;
+    intros a0 a1 Ha;
+    simpl;
+    [ | | assumption].
+  { apply op_proper;
+      [assumption |].
+    apply IHn.
+    apply op_proper;
+      assumption. }
+  { apply IHn.
+    apply op_proper;
+      assumption. }
+Qed.
+
+Context {semigroup: Semigroup equiv op}.
+Infix "==" := equiv (at level 60, no associativity).
+Infix "<o>" := op (at level 40, left associativity).
+
+Theorem semigroup_iter_op_succ (p: positive)(a: Carrier):
+  semigroup_iter_op (Pos.succ p) a == a <o> semigroup_iter_op p a.
+Proof.
+  generalize dependent a.
+  induction p;
+    intros a;
+    simpl;
+    [| reflexivity | reflexivity].
+  setoid_rewrite <- (semigroup_assoc equiv op).
+  apply IHp.
+Qed.
+
+Theorem semigroup_iter_op_add (p q: positive)(a: Carrier):
+  semigroup_iter_op (p + q) a ==
+    semigroup_iter_op p a <o> semigroup_iter_op q a.
+Proof.
+  generalize dependent a.
+  generalize dependent q.
+  induction p using Pos.peano_ind;
+    intros q a.
+  { rewrite Pos.add_1_l.
+    apply semigroup_iter_op_succ. }
+  { rewrite Pos.add_succ_l.
+    setoid_rewrite semigroup_iter_op_succ.
+    setoid_rewrite IHp.
+    symmetry.
+    apply (semigroup_assoc equiv op). }
+Qed.
+
+Theorem semigroup_iter_op_mul (p q: positive)(a: Carrier):
+  semigroup_iter_op (p * q) a ==
+    semigroup_iter_op p (semigroup_iter_op q a).
+Proof.
+  generalize dependent a.
+  generalize dependent q.
+  induction p using Pos.peano_ind;
+    intros q a;
+    simpl;
+    try reflexivity.
+  rewrite <- Pos.add_1_r.
+  rewrite Pos.mul_add_distr_r.
+  rewrite Pos.mul_1_l.
+  setoid_rewrite semigroup_iter_op_add.
+  simpl.
+  apply (semigroup_op_r equiv op).
+  apply IHp.
+Qed.
+
+Lemma semigroup_iter_op_comm_single (p: positive)(a b: Carrier):
+  a <o> b == b <o> a ->
+  a <o> semigroup_iter_op p b ==
+    semigroup_iter_op p b <o> a.
+Proof.
+  generalize dependent b.
+  generalize dependent a.
+  induction p using Pos.peano_ind;
+    intros a b Hab;
+    simpl;
+    [assumption |].
+  setoid_rewrite semigroup_iter_op_succ.
+  setoid_rewrite <- (semigroup_assoc equiv op).
+  setoid_rewrite Hab.
+  setoid_rewrite (semigroup_assoc equiv op).
+  apply (semigroup_op_l equiv op).
+  apply (IHp _ _ Hab).
+Qed.
+
+Lemma semigroup_iter_op_comm (p q: positive)(a b: Carrier):
+  a <o> b == b <o> a ->
+  semigroup_iter_op p a <o> semigroup_iter_op q b ==
+    semigroup_iter_op q b <o> semigroup_iter_op p a.
+Proof.
+  generalize dependent b.
+  generalize dependent a.
+  generalize dependent q.
+  induction p using Pos.peano_ind;
+    intros q a b Hab;
+    simpl.
+  { apply semigroup_iter_op_comm_single.
+    assumption. }
+  { setoid_rewrite semigroup_iter_op_succ.
+    setoid_rewrite <- (semigroup_assoc equiv op).
+    setoid_rewrite <- (semigroup_iter_op_comm_single _ _ _ Hab).
+    setoid_rewrite (semigroup_assoc equiv op).
+    apply (semigroup_op_l equiv op).
+    apply (IHp _ _ _ Hab). }
+Qed.
+
+Context (ident: Carrier).
+Context {monoid: Monoid equiv op ident}.
+
+Lemma semigroup_iter_op_ident (p: positive):
+  semigroup_iter_op p ident == ident.
+Proof.
+  induction p using Pos.peano_ind;
+    simpl;
+    [reflexivity |].
+  setoid_rewrite semigroup_iter_op_succ.
+  setoid_rewrite (monoid_ident_l equiv op ident).
+  assumption.
+Qed.
+
+Context (inv: Carrier -> Carrier).
+Context {inv_proper: Proper (equiv ==> equiv) inv}.
+Context {group: Group equiv op ident inv}.
+
+Definition group_iter_op (n: Z)(a: Carrier): Carrier :=
+  match n with
+  | Z0 => ident
+  | Zpos p => semigroup_iter_op p a
+  | Zneg p => semigroup_iter_op p (inv a)
+  end.
+
+Theorem group_iter_op_proper:
+  Proper (eq ==> equiv ==> equiv) group_iter_op.
+Proof.
+  intros m n ->.
+  destruct n;
+    intros a0 a1 Ha;
+    simpl;
+    try apply semigroup_iter_op_proper;
+    try reflexivity.
+  { assumption. }
+  { apply inv_proper.
+    assumption. }
+Qed.
+
+Lemma semigroup_iter_op_inv (p: positive)(a: Carrier):
+  semigroup_iter_op p (inv a) ==
+    inv (semigroup_iter_op p a).
+Proof.
+  generalize dependent a.
+  induction p using Pos.peano_ind;
+    intros a;
+    simpl;
+    [reflexivity |].
+  setoid_rewrite semigroup_iter_op_succ.
+  setoid_rewrite IHp.
+  setoid_rewrite <- (group_inv_op equiv op ident inv).
+  apply inv_proper.
+  symmetry.
+  apply semigroup_iter_op_comm_single.
+  reflexivity.
+Qed.
+
+Theorem group_iter_op_ident (n: Z):
+  group_iter_op n ident == ident.
+Proof.
+  destruct n as [| p | p];
+    simpl;
+    [reflexivity | |].
+  { apply semigroup_iter_op_ident. }
+  { setoid_rewrite semigroup_iter_op_inv.
+    setoid_rewrite semigroup_iter_op_ident.
+    apply (group_inv_ident equiv op ident inv). }
+Qed.
+
+Lemma semigroup_iter_op_pred_double (p: positive)(a: Carrier):
+  semigroup_iter_op (Pos.pred_double p) a ==
+    inv a <o> semigroup_iter_op p (a <o> a).
+Proof.
+  generalize dependent a.
+  induction p;
+    intros a;
+    simpl.
+  { transitivity (inv a <o> (a <o> a) <o> semigroup_iter_op p (a <o> a <o> (a <o> a)));
+      [| apply (semigroup_assoc equiv op)].
+    transitivity (inv a <o> a <o> a <o> semigroup_iter_op p (a <o> a <o> (a <o> a)));
+      [| apply (semigroup_op_r equiv op); apply (semigroup_assoc equiv op)].
+    setoid_rewrite (group_inv_l equiv op ident inv).
+    setoid_rewrite (monoid_ident_l equiv op ident).
+    reflexivity. }
+  { setoid_rewrite IHp.
+    transitivity (a <o> inv (a <o> a) <o> semigroup_iter_op p (a <o> a <o> (a <o> a)));
+      [symmetry; apply (semigroup_assoc equiv op) |].
+    apply (semigroup_op_r equiv op).
+    setoid_rewrite (group_inv_op equiv op ident inv).
+    setoid_rewrite <- (semigroup_assoc equiv op).
+    setoid_rewrite (group_inv_r equiv op ident inv).
+    apply (monoid_ident_l equiv op ident). }
+  { setoid_rewrite <- (semigroup_assoc equiv op).
+    setoid_rewrite (group_inv_l equiv op ident inv).
+    symmetry.
+    apply (monoid_ident_l equiv op ident). }
+Qed.
+
+Lemma semigroup_iter_op_inv_op (p: positive)(a b: Carrier):
+  semigroup_iter_op p (inv (a <o> b)) ==
+    semigroup_iter_op p (inv b <o> inv a).
+Proof.
+  apply semigroup_iter_op_proper;
+    [reflexivity |].
+  apply (group_inv_op equiv op ident inv).
+Qed.
+
+Lemma group_iter_op_succ_double (n: Z)(a: Carrier):
+  group_iter_op (Z.succ_double n) a ==
+    a <o> group_iter_op n (a <o> a).
+Proof.
+  destruct n;
+    simpl;
+    [| reflexivity |].
+  { symmetry.
+    apply (monoid_ident_r equiv op ident). }
+  { setoid_rewrite semigroup_iter_op_pred_double.
+    setoid_rewrite (group_inv_involute equiv op ident inv).
+    apply (semigroup_op_l equiv op).
+    symmetry.
+    apply semigroup_iter_op_inv_op. }
+Qed.
+
+Lemma group_iter_op_pred_double (n: Z)(a: Carrier):
+  group_iter_op (Z.pred_double n) a ==
+    inv a <o> group_iter_op n (a <o> a).
+Proof.
+  destruct n;
+    simpl;
+    [| apply semigroup_iter_op_pred_double |].
+  { symmetry.
+    apply (monoid_ident_r equiv op ident). }
+  { apply (semigroup_op_l equiv op).
+    symmetry.
+    apply semigroup_iter_op_inv_op. }
+Qed.
+
+Lemma group_iter_op_double (n: Z)(a: Carrier):
+  group_iter_op (Z.double n) a ==
+    group_iter_op n (a <o> a).
+Proof.
+  destruct n;
+    simpl;
+    [reflexivity | reflexivity |].
+  symmetry.
+  apply semigroup_iter_op_inv_op.
+Qed.
+
+Lemma group_iter_op_pos_sub (p q: positive)(a: Carrier):
+  group_iter_op (Z.pos_sub p q) a ==
+    semigroup_iter_op p a <o> semigroup_iter_op q (inv a).
+Proof.
+  generalize dependent a.
+  generalize dependent q.
+  induction p;
+    destruct q;
+    intros a;
+    simpl.
+  { setoid_rewrite group_iter_op_double.
+    setoid_rewrite IHp.
+    setoid_rewrite <- (semigroup_assoc equiv op).
+    transitivity (a <o> semigroup_iter_op p (a <o> a) <o> inv a <o> semigroup_iter_op q (inv (a <o> a)));
+      [| apply (semigroup_op_l equiv op)].
+    { apply (semigroup_op_r equiv op).
+      setoid_rewrite (semigroup_assoc equiv op).
+      transitivity (a <o> (inv a <o> semigroup_iter_op p (a <o> a)));
+        [| apply (semigroup_op_l equiv op); apply semigroup_iter_op_comm_single].
+      { setoid_rewrite <- (semigroup_assoc equiv op).
+        setoid_rewrite (group_inv_r equiv op ident inv).
+        symmetry.
+        apply (monoid_ident_l equiv op ident). }
+      { apply (group_move_r equiv op ident inv).
+        setoid_rewrite (semigroup_assoc equiv op).
+        symmetry.
+        apply (group_move_l equiv op ident inv).
+        symmetry.
+        apply (semigroup_assoc equiv op). } }
+    { apply semigroup_iter_op_inv_op. } }
+  { setoid_rewrite group_iter_op_succ_double.
+    setoid_rewrite IHp.
+    setoid_rewrite <- (semigroup_assoc equiv op).
+    apply (semigroup_op_l equiv op).
+    apply semigroup_iter_op_inv_op. }
+  { apply (group_move_r equiv op ident inv).
+    symmetry.
+    apply semigroup_iter_op_comm_single.
+    symmetry.
+    apply (semigroup_assoc equiv op). }
+  { setoid_rewrite group_iter_op_pred_double.
+    setoid_rewrite IHp.
+    transitivity (semigroup_iter_op p (a <o> a) <o> inv a <o> semigroup_iter_op q (inv a <o> inv a));
+      [| apply (semigroup_assoc equiv op)].
+    transitivity (inv a <o> semigroup_iter_op p (a <o> a) <o> semigroup_iter_op q (inv a <o> inv a));
+      [| apply (semigroup_op_r equiv op)].
+    { setoid_rewrite <- (semigroup_assoc equiv op).
+      apply (semigroup_op_l equiv op).
+      apply semigroup_iter_op_inv_op. }
+    { apply semigroup_iter_op_comm_single.
+      symmetry;
+      apply (group_move_l equiv op ident inv);
+      symmetry.
+      repeat setoid_rewrite <- (semigroup_assoc equiv op).
+      apply (group_move_r equiv op ident inv).
+      reflexivity. } }
+  { setoid_rewrite group_iter_op_double.
+    setoid_rewrite IHp.
+    apply (semigroup_op_l equiv op).
+    apply semigroup_iter_op_inv_op. }
+  { setoid_rewrite semigroup_iter_op_pred_double.
+    apply semigroup_iter_op_comm_single.
+    setoid_rewrite <- (semigroup_assoc equiv op).
+    setoid_rewrite (group_inv_l equiv op ident inv).
+    setoid_rewrite (monoid_ident_l equiv op ident).
+    apply (group_move_r equiv op ident inv).
+    reflexivity. }
+  { setoid_rewrite <- (semigroup_assoc equiv op).
+    setoid_rewrite (group_inv_r equiv op ident inv).
+    symmetry.
+    apply (monoid_ident_l equiv op ident). }
+  { setoid_rewrite semigroup_iter_op_pred_double.
+    setoid_rewrite (group_inv_involute equiv op ident inv).
+    reflexivity. }
+  { symmetry.
+    apply (group_inv_r equiv op ident inv). }
+Qed.
+
+Theorem group_iter_op_add (m n: Z)(a: Carrier):
+  group_iter_op (m + n) a ==
+    group_iter_op m a <o> group_iter_op n a.
+Proof.
+  generalize dependent a.
+  destruct m as [| p | p],
+    n as [| q | q];
+    intros a;
+    simpl;
+    try (symmetry; apply (monoid_ident_l equiv op ident));
+    try (symmetry; apply (monoid_ident_r equiv op ident));
+    try apply semigroup_iter_op_add.
+  { apply group_iter_op_pos_sub. }
+  { setoid_rewrite group_iter_op_pos_sub.
+    apply semigroup_iter_op_comm.
+    setoid_rewrite (group_inv_l equiv op ident inv).
+    apply (group_inv_r equiv op ident inv). }
+Qed.
+
+Theorem group_iter_op_neg (n: Z)(a: Carrier):
+  group_iter_op (-n) a == group_iter_op n (inv a).
+Proof.
+  destruct n as [| p | p];
+    simpl;
+    [reflexivity | reflexivity |].
+  symmetry.
+  apply semigroup_iter_op_proper;
+    [reflexivity |].
+  apply (group_inv_involute equiv op ident inv).
+Qed.
+
+Theorem group_iter_op_inv (n: Z)(a: Carrier):
+  group_iter_op n (inv a) == inv (group_iter_op n a).
+Proof.
+  destruct n;
+    simpl.
+  { symmetry;
+    apply (group_inv_ident equiv op ident inv). }
+  { apply semigroup_iter_op_inv. }
+  { apply semigroup_iter_op_inv. }
+Qed.
+
+Theorem group_iter_op_comm (m n: Z)(a b: Carrier):
+  a <o> b == b <o> a ->
+  group_iter_op m a <o> group_iter_op n b ==
+    group_iter_op n b <o> group_iter_op m a.
+Proof.
+  intros Hab.
+  destruct m as [| p | p], n as [| q | q];
+    simpl;
+    try (setoid_rewrite (monoid_ident_r equiv op ident));
+    try (setoid_rewrite (monoid_ident_l equiv op ident));
+    try reflexivity.
+  { apply semigroup_iter_op_comm;
+      assumption. }
+  { apply semigroup_iter_op_comm.
+    apply (group_move_l equiv op ident inv).
+    symmetry.
+    setoid_rewrite <- (semigroup_assoc equiv op).
+    apply (group_move_r equiv op ident inv).
+    assumption. }
+  { apply semigroup_iter_op_comm.
+    apply (group_move_r equiv op ident inv).
+    symmetry.
+    setoid_rewrite (semigroup_assoc equiv op).
+    apply (group_move_l equiv op ident inv).
+    assumption. }
+  { apply semigroup_iter_op_comm.
+    setoid_rewrite <- (group_inv_op equiv op ident inv).
+    apply inv_proper.
+    symmetry.
+    assumption. }
+Qed.
+
+Theorem group_iter_op_mul (m n: Z)(a: Carrier):
+  group_iter_op (m * n) a ==
+    group_iter_op m (group_iter_op n a).
+Proof.
+  destruct m as [| p | p].
+  { rewrite Z.mul_0_l.
+    simpl.
+    reflexivity. }
+  { destruct n as [| q | q];
+      simpl.
+    { symmetry;
+        apply semigroup_iter_op_ident. }
+    { apply semigroup_iter_op_mul. }
+    { apply semigroup_iter_op_mul. } }
+  { destruct n as [| q | q];
+      simpl.
+    { symmetry.
+      setoid_rewrite semigroup_iter_op_inv.
+      setoid_rewrite semigroup_iter_op_ident.
+      apply (group_inv_ident equiv op ident inv). }
+    { setoid_rewrite semigroup_iter_op_mul.
+      apply semigroup_iter_op_proper;
+        [reflexivity |].
+      apply semigroup_iter_op_inv. }
+    { setoid_rewrite semigroup_iter_op_mul.
+      apply semigroup_iter_op_proper;
+        [reflexivity |].
+      symmetry.
+      setoid_rewrite semigroup_iter_op_inv.
+      setoid_rewrite (group_inv_involute equiv op ident inv).
+      reflexivity. } }
+Qed.
+End OpIterations.
