theories/Modules.v
@@ -1,8 +1,6 @@
 Require Import Coq.Relations.Relations.
-Require Import Coq.Classes.RelationClasses.
-Require Import Coq.Classes.Morphisms.
-From algebra Require Import Groups.
-From algebra Require Import AbelianGroups CommRings.
+From Coq.Classes Require Import RelationClasses Morphisms.
+From algebra Require Import AbelianGroups Groups CommRings.
 
 Section Modules.
 Context {R: Type}.
@@ -29,31 +27,31 @@ Context {Magroup: AbelianGroup Mequiv Madd Mzero Mminus}.
 Context (action: R -> M -> M).
 Context {action_proper: Proper (Requiv ==> Mequiv ==> Mequiv) action}.
 
-Infix "&" := Requiv (at level 60, no associativity).
+Infix "=R=" := Requiv (at level 60, no associativity).
 Infix "[+]" := Radd (at level 50, left associativity).
 Infix "[*]" := Rmul (at level 40, left associativity).
-Infix "~" := Mequiv (at level 60, no associativity).
+Infix "=M=" := Mequiv (at level 60, no associativity).
 Infix "<+>" := Madd (at level 50, left associativity).
 Infix "<.>" := action (at level 40, no associativity).
 
 Class Module_ := {
   module_distrib_Madd:
     forall (r: R)(a b: M),
-      r <.> (a <+> b) ~ r <.> a <+> r <.> b;
+      r <.> (a <+> b) =M= r <.> a <+> r <.> b;
   module_distrib_Radd:
     forall (r s: R)(a: M),
-      (r [+] s) <.> a ~ r <.> a <+> s <.> a;
+      (r [+] s) <.> a =M= r <.> a <+> s <.> a;
   module_distrib_Rmul:
     forall (r s: R)(a: M),
-      (r [*] s) <.> a ~ r <.> (s <.> a);
+      (r [*] s) <.> a =M= r <.> (s <.> a);
   module_Rone:
-    forall (a: M), Rone <.> a ~ a;
+    forall (a: M), Rone <.> a =M= a;
 }.
 
 Context `{module: Module_}.
 
 Lemma module_op_l (a b: M):
-  a ~ b -> forall (r: R), r <.> a ~ r <.> b.
+  a =M= b -> forall (r: R), r <.> a =M= r <.> b.
 Proof.
   intros Hab r.
   apply action_proper;
@@ -62,7 +60,7 @@ Proof.
 Qed.
 
 Lemma module_op_r (r s: R):
-  r & s -> forall (a: M), r <.> a ~ s <.> a.
+  r =R= s -> forall (a: M), r <.> a =M= s <.> a.
 Proof.
   intros Hrs a.
   apply action_proper;
@@ -71,57 +69,46 @@ Proof.
 Qed.
 
 Theorem module_0_l (a: M):
-  Rzero <.> a ~ Mzero.
+  Rzero <.> a =M= Mzero.
 Proof.
   apply (group_idemp_ident Mequiv Madd Mzero Mminus).
-  transitivity ((Rzero [+] Rzero) <.> a);
-    [symmetry; apply module_distrib_Radd |].
+  setoid_rewrite <- module_distrib_Radd.
   apply module_op_r.
   apply (group_ident_r Requiv Radd Rzero Rminus).
 Qed.
 
 Theorem module_0_r (r: R):
-  r <.> Mzero ~ Mzero.
+  r <.> Mzero =M= Mzero.
 Proof.
   apply (group_idemp_ident Mequiv Madd Mzero Mminus).
-  transitivity (r <.> (Mzero <+> Mzero));
-    [symmetry; apply module_distrib_Madd |].
+  setoid_rewrite <- module_distrib_Madd.
   apply module_op_l.
   apply (group_ident_r Mequiv Madd Mzero Mminus).
 Qed.
 
 Theorem module_minus_l (r: R)(a: M):
-  (Rminus r) <.> a ~ Mminus (r <.> a).
+  (Rminus r) <.> a =M= Mminus (r <.> a).
 Proof.
   apply (group_inv_r_unique Mequiv Madd Mzero Mminus).
-  transitivity ((r [+] Rminus r) <.> a);
-    [symmetry; apply module_distrib_Radd |].
-  transitivity (Rzero <.> a);
-    [| apply module_0_l].
-  apply module_op_r.
-  apply (group_inv_r Requiv Radd Rzero Rminus).
+  setoid_rewrite <- module_distrib_Radd.
+  setoid_rewrite (group_inv_r Requiv Radd Rzero Rminus).
+  apply module_0_l.
 Qed.
 
 Theorem module_minus_r (r: R)(a: M):
-  r <.> Mminus a ~ Mminus (r <.> a).
+  r <.> Mminus a =M= Mminus (r <.> a).
 Proof.
   apply (group_inv_r_unique Mequiv Madd Mzero Mminus).
-  transitivity (r <.> (a <+> Mminus a));
-    [symmetry; apply module_distrib_Madd |].
-  transitivity (r <.> Mzero);
-    [| apply module_0_r].
-  apply module_op_l.
-  apply (group_inv_r Mequiv Madd Mzero Mminus).
+  setoid_rewrite <- (module_distrib_Madd).
+  setoid_rewrite (group_inv_r Mequiv Madd Mzero Mminus).
+  apply module_0_r.
 Qed.
 
 Theorem module_minus_minus (r: R)(a: M):
-  Rminus r <.> Mminus a ~ r <.> a.
+  Rminus r <.> Mminus a =M= r <.> a.
 Proof.
-  transitivity (Mminus (r <.> Mminus a));
-    [apply module_minus_l |].
-  transitivity (Mminus (Mminus (r <.> a)));
-    [| apply (group_inv_involute Mequiv Madd Mzero Mminus)].
-  apply Mminus_proper.
-  apply module_minus_r.
+  setoid_rewrite module_minus_l.
+  setoid_rewrite module_minus_r.
+  apply (group_inv_involute Mequiv Madd Mzero Mminus).
 Qed.
 End Modules.
