theories/Rings.v
@@ -1,6 +1,5 @@
 Require Import Coq.Relations.Relations.
-Require Import Coq.Classes.RelationClasses.
-Require Import Coq.Classes.Morphisms.
+From Coq.Classes Require Import RelationClasses Morphisms.
 From algebra Require Import Semigroups Monoids Groups AbelianGroups.
 
 Section Rings.
@@ -15,7 +14,7 @@ Context {minus_proper: Proper (equiv ==> equiv) minus}.
 Context (mul: Carrier -> Carrier -> Carrier).
 Context {mul_proper: Proper (equiv ==> equiv ==> equiv) mul}.
 
-Infix "~" := equiv (at level 60, no associativity).
+Infix "==" := equiv (at level 60, no associativity).
 Infix "<+>" := add (at level 50, left associativity).
 Infix "<*>" := mul (at level 40, left associativity).
 
@@ -24,66 +23,55 @@ Class Ring := {
   ring_mul_semigroup :> Semigroup equiv mul;
   ring_distrib_l:
     forall (a b c: Carrier),
-      a <*> (b <+> c) ~ a <*> b <+> a <*> c;
+      a <*> (b <+> c) == a <*> b <+> a <*> c;
   ring_distrib_r:
     forall (a b c: Carrier),
-      (b <+> c) <*> a ~ b <*> a <+> c <*> a;
+      (b <+> c) <*> a == b <*> a <+> c <*> a;
 }.
 
 Context {ring: Ring}.
 
 Theorem ring_mul_0_l (a: Carrier):
-  zero <*> a ~ zero.
+  zero <*> a == zero.
 Proof.
   apply (group_idemp_ident equiv add zero minus).
-  transitivity ((zero <+> zero) <*> a);
-    [symmetry; apply ring_distrib_r |].
-  apply (semigroup_op_r equiv mul).
-  apply (monoid_ident_r equiv add zero).
+  setoid_rewrite <- ring_distrib_r.
+  setoid_rewrite (monoid_ident_r equiv add zero).
+  reflexivity.
 Qed.
 
 Theorem ring_mul_0_r (a: Carrier):
-  a <*> zero ~ zero.
+  a <*> zero == zero.
 Proof.
   apply (group_idemp_ident equiv add zero minus).
-  transitivity (a <*> (zero <+> zero));
-    [symmetry; apply ring_distrib_l |].
-  apply (semigroup_op_l equiv mul).
-  apply (monoid_ident_r equiv add zero).
+  setoid_rewrite <- ring_distrib_l.
+  setoid_rewrite (monoid_ident_r equiv add zero).
+  reflexivity.
 Qed.
 
 Theorem ring_mul_minus_l (a b: Carrier):
-  (minus a) <*> b ~ minus (a <*> b).
+  (minus a) <*> b == minus (a <*> b).
 Proof.
   apply (group_inv_r_unique equiv add zero minus).
-  transitivity ((a <+> minus a) <*> b);
-    [symmetry; apply ring_distrib_r |].
-  transitivity (zero <*> b);
-    [apply (semigroup_op_r equiv mul);
-      apply (group_inv_r equiv add zero minus) |].
+  setoid_rewrite <- ring_distrib_r.
+  setoid_rewrite (group_inv_r equiv add zero minus).
   apply ring_mul_0_l.
 Qed.
 
 Theorem ring_mul_minus_r (a b: Carrier):
-  a <*> (minus b) ~ minus (a <*> b).
+  a <*> (minus b) == minus (a <*> b).
 Proof.
   apply (group_inv_r_unique equiv add zero minus).
-  transitivity (a <*> (b <+> minus b));
-    [symmetry; apply ring_distrib_l |].
-  transitivity (a <*> zero);
-    [apply (semigroup_op_l equiv mul);
-      apply (group_inv_r equiv add zero minus) |].
+  setoid_rewrite <- ring_distrib_l.
+  setoid_rewrite (group_inv_r equiv add zero minus).
   apply ring_mul_0_r.
 Qed.
 
 Theorem ring_mul_minus_minus (a b: Carrier):
-  (minus a) <*> (minus b) ~ a <*> b.
+  (minus a) <*> (minus b) == a <*> b.
 Proof.
-  transitivity (minus (a <*> minus b));
-    [apply ring_mul_minus_l |].
-  transitivity (minus (minus (a <*> b)));
-    [apply minus_proper;
-      apply ring_mul_minus_r |].
+  setoid_rewrite ring_mul_minus_l.
+  setoid_rewrite ring_mul_minus_r.
   apply (group_inv_involute equiv add zero minus).
 Qed.
 End Rings.
